interface for Benton2004.RHL

examples/rel/Benton2004.RHL.fsti
@@ -14,78 +14,118 @@
    limitations under the License.
 *)
 module Benton2004.RHL
+include Benton2004
 
 (* Relational Hoare Logic (Section 4) *)
 
-let gsubst_gconst (#t: Type0) (n: t) (x: var) (side: pos) (ge' : gexp int): Lemma
+type gexp (t: Type0) = heap -> heap -> GTot t
+
+let gconst (#t: Type0) (n: t) : gexp t =
+  let g _ _ : GTot t = n in
+  g
+
+type pos =
+  | Left
+  | Right
+
+let gvar (x: var) (side: pos) : GTot (gexp int) =
+  let g s1 s2 : GTot int = sel (match side with Left -> s1 | Right -> s2) x in
+  g
+
+let gop (#from #to: Type0) (op: (from -> from -> GTot to)) (e1 e2: gexp from) : GTot (gexp to) =
+  let g s1 s2 : GTot to = op (e1 s1 s2) (e2 s1 s2) in
+  g
+
+let gnot (e: gexp bool) : GTot (gexp bool) =
+  let g s1 s2 = not (e s1 s2) in
+  g
+
+(* Substitution: Lemma 3 al. 1, 2 *)
+
+let gsubst (#t: Type0) (ge: gexp t) (x: var) (side: pos) (ge': gexp int) : gexp t =
+  let g s1 s2 : GTot t =
+    let v' = ge' s1 s2 in
+    match side with
+    | Left -> ge (upd s1 x v') s2
+    | Right -> ge s1 (upd s2 x v')
+  in
+  g
+
+val gsubst_gconst (#t: Type0) (n: t) (x: var) (side: pos) (ge' : gexp int): Lemma
   (forall h1 h2. (gsubst (gconst n) x side ge') h1 h2 == (gconst n) h1 h2)
   [SMTPat (gsubst (gconst n) x side ge')]
-= ()
 
-let gsubst_gvar_same (x: var) (side: pos) (ge': gexp int) : Lemma
+val gsubst_gvar_same (x: var) (side: pos) (ge': gexp int) : Lemma
   (forall h1 h2. (gsubst (gvar x side) x side ge') h1 h2 == ge' h1 h2)
   [SMTPat (gsubst (gvar x side) x side ge')]
-= ()
 
-let gsubst_gvar_other (x x': var) (side side': pos) (ge': gexp int) : Lemma
+val gsubst_gvar_other (x x': var) (side side': pos) (ge': gexp int) : Lemma
   (requires (x <> x' \/ side <> side'))
   (ensures  (forall h1 h2. (gsubst (gvar x side) x' side' ge') h1 h2 == (gvar x side) h1 h2))
   [SMTPat (gsubst (gvar x side) x' side' ge')]
-=  ()
 
-let gsubst_gop (#from #to: Type0) (op: (from -> from -> GTot to)) (ge1 ge2: gexp from) (x: var) (side: pos) (ge': gexp int) : Lemma
+val gsubst_gop (#from #to: Type0) (op: (from -> from -> GTot to)) (ge1 ge2: gexp from) (x: var) (side: pos) (ge': gexp int) : Lemma
   (forall h1 h2. (gsubst (gop op ge1 ge2) x side ge') h1 h2 ==
             (gop op (gsubst ge1 x side ge') (gsubst ge2 x side ge')) h1 h2)
   [SMTPat (gsubst (gop op ge1 ge2) x side ge')]
-= ()
 
-let holds_interp
+(* 4.1.3 Inference rules *)
+
+let interp (ge: gexp bool) : GTot sttype =
+  let g s1 s2 : GTot Type0 = ge s1 s2 == true in
+  g
+
+val holds_interp
   (ge: gexp bool)
   (s1 s2: heap)
 : Lemma
   (holds (interp ge) s1 s2 <==> ge s1 s2 == true)
   [SMTPat (holds (interp ge) s1 s2)]
-= holds_equiv (interp ge) s1 s2
 
-let exec_equiv
+val exec_equiv
   (p p' : gexp bool)
   (f f' : computation)
 : GTot Type0
-= Benton2004.exec_equiv (interp p) (interp p') f f'
 
-let exec_equiv_elim
+val exec_equiv_elim
   (p p' : gexp bool)
   (f f' : computation)
 : Lemma
   (requires (exec_equiv p p' f f'))
   (ensures (Benton2004.exec_equiv (interp p) (interp p') f f'))
-= ()
 
-let r_skip
+val r_skip
   (p: gexp bool)
 : Lemma
   (exec_equiv p p skip skip)
   [SMTPat (exec_equiv p p skip skip)]
-= d_skip (interp p)
 
-let exp_to_gexp_const
+let exp_to_gexp
+  (#t: Type0)
+  (e: exp t)
+  (side: pos)
+: GTot (gexp t)
+= let g s1 s2 : GTot t =
+    fst (reify_exp e (match side with | Left -> s1 | Right -> s2))
+  in
+  g
+
+val exp_to_gexp_const
   (#t: Type0)
   (c: t)
   (side: pos)
 : Lemma
   (forall h1 h2. (exp_to_gexp (const c) side) h1 h2 == (gconst c) h1 h2)
   [SMTPat (exp_to_gexp (const c) side)]
-= ()
 
-let exp_to_gexp_evar
+val exp_to_gexp_evar
   (x: var)
   (side: pos)
 : Lemma
   (forall h1 h2. (exp_to_gexp (evar x) side) h1 h2 == (gvar x side) h1 h2)
   [SMTPat (exp_to_gexp (evar x) side)]
-= ()
 
-let exp_to_gexp_eop
+val exp_to_gexp_eop
   (#from #to: Type0)
   (op: (from -> from -> Tot to))
   (e1 e2: exp from)
@@ -93,60 +133,67 @@ let exp_to_gexp_eop
 : Lemma
   (forall h1 h2. (exp_to_gexp (eop op e1 e2) side) h1 h2 == (gop op (exp_to_gexp e1 side) (exp_to_gexp e2 side)) h1 h2)
   [SMTPat (exp_to_gexp (eop op e1 e2) side)]
-= ()
 
-#set-options "--z3rlimit 2048 --max_fuel 8 --max_ifuel 8"
+let gand (b1 b2 : gexp bool) : GTot (gexp bool) =
+  gop op_AmpAmp b1 b2
 
-let holds_gand (b1 b2 : gexp bool) : Lemma
+val holds_gand (b1 b2 : gexp bool) : Lemma
   (forall s1 s2 . holds (interp (gand b1 b2)) s1 s2 <==> holds (interp b1) s1 s2 /\ holds (interp b2) s1 s2)
   [SMTPat (holds (interp (gand b1 b2)))]
-= ()
 
-let gsubst_gand (b1 b2: gexp bool) x side e : Lemma
+val gsubst_gand (b1 b2: gexp bool) (x:_) (side:_) (e:_) : Lemma
   (forall h1 h2. (gsubst (gand b1 b2) x side e) h1 h2 == (gand (gsubst b1 x side e) (gsubst b2 x side e)) h1 h2)
   [SMTPat (gsubst (gand b1 b2) x side e)]
-= ()
 
-let holds_gor (b1 b2 : gexp bool) : Lemma
+let gor (b1 b2 : gexp bool) : GTot (gexp bool) =
+  gop op_BarBar b1 b2
+
+val holds_gor (b1 b2 : gexp bool) : Lemma
   (forall s1 s2 . holds (interp (gor b1 b2)) s1 s2 <==> holds (interp b1) s1 s2 \/ holds (interp b2) s1 s2)
   [SMTPat (holds (interp (gor b1 b2)))]
-= ()
 
-let gsubst_gor (b1 b2: gexp bool) x side e : Lemma
+val gsubst_gor (b1 b2: gexp bool) (x:_) (side:_) (e:_) : Lemma
   (forall h1 h2. (gsubst (gor b1 b2) x side e) h1 h2 == (gor (gsubst b1 x side e) (gsubst b2 x side e)) h1 h2)
   [SMTPat (gsubst (gor b1 b2) x side e)]
-= ()
 
-let holds_gnot (b: gexp bool) : Lemma
+val holds_gnot (b: gexp bool) : Lemma
   (forall s1 s2 . holds (interp (gnot b)) s1 s2 <==> ~ (holds (interp b) s1 s2))
   [SMTPat (holds (interp (gnot b)))]
-= ()
 
-let holds_geq (#t: eqtype) (e1 e2 : gexp t) : Lemma
+let geq
+  (#t: eqtype)
+  (e1 e2 : gexp t)
+: GTot (gexp bool)
+= gop op_Equality e1 e2
+
+val holds_geq (#t: eqtype) (e1 e2 : gexp t) : Lemma
   (forall s1 s2 . holds (interp (geq e1 e2)) s1 s2 <==> e1 s1 s2 == e2 s1 s2)
   [SMTPat (holds (interp (geq e1 e2)))]
-= ()
 
-let gsubst_geq (#t: eqtype) (b1 b2: gexp t) x side e : Lemma
+val gsubst_geq (#t: eqtype) (b1 b2: gexp t) (x:_) (side:_) (e:_) : Lemma
   (forall h1 h2. (gsubst (geq b1 b2) x side e) h1 h2 == (geq (gsubst b1 x side e) (gsubst b2 x side e)) h1 h2)
   [SMTPat (gsubst (geq b1 b2) x side e)]
-= ()
 
-let holds_exp_to_gexp_left
+val holds_exp_to_gexp_left
   (e: exp bool)
 : Lemma
   (forall s1 s2 . holds (interp (exp_to_gexp e Left)) s1 s2 <==> fst (reify_exp e s1) == true)
   [SMTPat (holds (interp (exp_to_gexp e Left)))]
-= ()
 
-let holds_exp_to_gexp_right
+val holds_exp_to_gexp_right
   (e: exp bool)
 : Lemma
   (forall s1 s2 . holds (interp (exp_to_gexp e Right)) s1 s2 <==> fst (reify_exp e s2) == true)
   [SMTPat (holds (interp (exp_to_gexp e Right)))]
-= ()
 
-let holds_r_if_precond_true
+let r_if_precond_true
+  (b b': exp bool)
+  (c c' d d' : computation)
+  (p p' : gexp bool)
+: GTot (gexp bool)
+= gand p (gand (exp_to_gexp b Left) (exp_to_gexp b' Right))
+
+val holds_r_if_precond_true
   (b b': exp bool)
   (c c' d d' : computation)
   (p p' : gexp bool)
@@ -157,9 +204,15 @@ let holds_r_if_precond_true
     fst (reify_exp b s1) == true /\
     fst (reify_exp b' s2) == true
   ))
-= ()
 
-let holds_r_if_precond_false
+let r_if_precond_false
+  (b b': exp bool)
+  (c c' d d' : computation)
+  (p p' : gexp bool)
+: GTot (gexp bool)
+= gand p (gnot (gor (exp_to_gexp b Left) (exp_to_gexp b' Right)))
+
+val holds_r_if_precond_false
   (b b': exp bool)
   (c c' d d' : computation)
   (p p' : gexp bool)
@@ -169,9 +222,15 @@ let holds_r_if_precond_false
     holds (interp p) s1 s2 /\
     ( ~ (fst (reify_exp b s1) == true \/ fst (reify_exp b' s2) == true))   
   ))
-= ()  
 
-let holds_r_if_precond
+let r_if_precond
+  (b b': exp bool)
+  (c c' d d' : computation)
+  (p p' : gexp bool)
+: GTot (gexp bool)
+= gand p (geq (exp_to_gexp b Left) (exp_to_gexp b' Right))
+
+val holds_r_if_precond
   (b b': exp bool)
   (c c' d d' : computation)
   (p p' : gexp bool)
@@ -181,9 +240,8 @@ let holds_r_if_precond
     holds (interp p) s1 s2 /\
     fst (reify_exp b s1) == fst (reify_exp b' s2)
   ))
-= ()
 
-let r_if
+val r_if
   (b b': exp bool)
   (c c' d d' : computation)
   (p p' : gexp bool)
@@ -207,11 +265,8 @@ let r_if
       (ifthenelse b c d)
       (ifthenelse b' c' d')
   ))
-= holds_r_if_precond_true b b' c c' d d' p p';
-  holds_r_if_precond_false b b' c c' d d' p p';
-  holds_r_if_precond b b' c c' d d' p p'
 
-let r_seq
+val r_seq
   (p0 p1 p2 : gexp bool)
   (c01 c01' c12 c12' : computation)
 : Lemma
@@ -227,9 +282,8 @@ let r_seq
     [SMTPat (exec_equiv p0 p2 (seq c01 c12) (seq c01' c12')); SMTPat (exec_equiv p1 p2 c12 c12')];
     [SMTPat (exec_equiv p0 p1 c01 c01'); SMTPat (exec_equiv p1 p2 c12 c12')];
   ]]
-= d_seq (interp p0) (interp p1) (interp p2) c01 c01' c12 c12'
 
-let r_ass
+val r_ass
   (x y: var)
   (e e' : exp int)
   (p: gexp bool)
@@ -240,15 +294,15 @@ let r_ass
     (assign x e)
     (assign y e')
   )
-= ()
 
-let included_alt (p1 p2 : gexp bool) : Lemma
+let included (p1 p2: gexp bool) : GTot Type0 =
+  Benton2004.included (interp p1) (interp p2)
+
+val included_alt (p1 p2 : gexp bool) : Lemma
   (included p1 p2 <==> (forall s1 s2 . p1 s1 s2 == true ==> p2 s1 s2 == true))
   [SMTPat (included p1 p2)]
-= assert (forall s1 s2 . holds (interp p1) s1 s2 <==> p1 s1 s2 == true);
-  assert (forall s1 s2 . holds (interp p2) s1 s2 <==> p2 s1 s2 == true)
 
-let r_sub
+val r_sub
   (p1 p2 p1' p2' : gexp bool)
   (f f' : computation)
 : Lemma
@@ -259,9 +313,8 @@ let r_sub
   ))
   (ensures (exec_equiv p1' p2' f f'))
   [SMTPat (exec_equiv p1' p2' f f'); SMTPat (exec_equiv p1 p2 f f')]
-= d_csub (interp p1) (interp p2) (interp p1') (interp p2') f f'
 
-let rec r_while_terminates'
+val r_while_terminates'
   (b b' : exp bool)
   (c c' : computation)
   (phi phi_c phi_c': gexp bool)
@@ -280,57 +333,23 @@ let rec r_while_terminates'
     terminates_on (reify_computation (while b' c')) s0'
   ))
   (decreases fuel)
-= let f = reify_computation (while b c) in
-  let f' = reify_computation (while b' c') in
-  let fc = reify_computation c in
-  let fc' = reify_computation c' in
-  if fst (reify_exp b s0)
-  then begin
-//    let s1 = snd (reify_computation c fuel s0) in
-    assert (holds (interp (gand phi (gand (exp_to_gexp b Left) (exp_to_gexp b' Right)))) s0 s0');
-    assert (terminates_on (fc') s0');
-    let g
-      (fuel0 : nat)
-    : Lemma
-      (requires (fst (fc' fuel0 s0') == true))
-      (ensures (terminates_on (f') s0'))
-    = let s1 = snd (fc fuel s0) in
-      let s1' = snd (fc' fuel0 s0') in
-      let fuel1 = fuel + fuel0 in
-      assert (fc fuel1 s0 == fc fuel s0);
-      assert (fc' fuel1 s0' == fc' fuel0 s0');
-      r_while_terminates' b b' c c' phi phi_c phi_c' s1 s1' (fuel - 1);
-      let g'
-        (fuel2 : nat)
-      : Lemma
-        (requires (fst (f' fuel2 s1') == true))
-        (ensures (terminates_on (f') s0'))
-      = let fuel3 = fuel0 + fuel2 + 1 in
-        assert (f' (fuel3 - 1) s1' == f' fuel2 s1');
-        assert (fc' fuel3 s0' == fc' fuel0 s0');
-        assert (fst (f' fuel3 s0') == true)
-      in
-      Classical.forall_intro (Classical.move_requires g')
-    in
-    Classical.forall_intro (Classical.move_requires g)
-  end else ()
 
-let holds_interp_flip (phi: gexp bool) : Lemma
+let flip (phi: gexp bool) : Tot (gexp bool) =
+  let g s1 s2 = phi s2 s1 in
+  g
+
+val holds_interp_flip (phi: gexp bool) : Lemma
   (forall s1 s2 . holds (interp (flip phi)) s1 s2 <==> holds (Benton2004.flip (interp phi)) s1 s2)
   [SMTPat (holds (interp (flip phi)))]
-= Benton2004.holds_flip (interp phi)
 
-let exec_equiv_flip
+val exec_equiv_flip
   (p p': gexp bool)
   (f f' : computation)
 : Lemma
   (exec_equiv (flip p) (flip p') f f' <==> exec_equiv p p' f' f)
   [SMTPat (exec_equiv (flip p) (flip p') f f')]
-= holds_interp_flip p;
-  holds_interp_flip p';
-  exec_equiv_flip (interp p) (interp p') f f'
 
-let r_while_terminates
+val r_while_terminates
   (b b' : exp bool)
   (c c' : computation)
   (p: gexp bool)
@@ -344,13 +363,8 @@ let r_while_terminates
     terminates_on (reify_computation (while b c)) s0 <==>
     terminates_on (reify_computation (while b' c')) s0'
   ))
-= let phi = gand p (geq (exp_to_gexp b Left) (exp_to_gexp b' Right)) in
-  let phi_c = gand p (gand (exp_to_gexp b Left) (exp_to_gexp b' Right)) in
-  let phi_c' = gand p (geq (exp_to_gexp b Left) (exp_to_gexp b' Right)) in
-  Classical.forall_intro (Classical.move_requires (r_while_terminates' b b' c c' phi phi_c phi_c' s0 s0'));
-  Classical.forall_intro (Classical.move_requires (r_while_terminates' b' b c' c (flip phi) (flip phi_c) (flip phi_c') s0' s0))
 
-let rec r_while_correct
+val r_while_correct
   (b b' : exp bool)
   (c c' : computation)
   (p: gexp bool)
@@ -367,18 +381,8 @@ let rec r_while_correct
     holds (interp (gand p (gnot (gor (exp_to_gexp b Left) (exp_to_gexp b' Right))))) (snd (reify_computation (while b c) fuel s0)) (snd (reify_computation (while b' c') fuel s0'))
   ))
   (decreases fuel)
-= let f = reify_computation (while b c) in
-  let f' = reify_computation (while b' c') in
-  let fc = reify_computation c in
-  let fc' = reify_computation c' in
-  if fst (reify_exp b s0)
-  then
-    let s1 = snd (fc fuel s0) in
-    let s1' = snd (fc' fuel s0') in
-    r_while_correct b b' c c' p s1 s1' (fuel - 1)
-  else ()
 
-let rec r_while
+val r_while
   (b b' : exp bool)
   (c c' : computation)
   (p: gexp bool)
@@ -389,45 +393,27 @@ let rec r_while
   (ensures (
     exec_equiv (gand p (geq (exp_to_gexp b Left) (exp_to_gexp b' Right))) (gand p (gnot (gor (exp_to_gexp b Left) (exp_to_gexp b' Right)))) (while b c) (while b' c')
   ))
-= let g (s0 s0':heap)
-  :Lemma ((exec_equiv (gand p (gand (exp_to_gexp b Left) (exp_to_gexp b' Right))) (gand p (geq (exp_to_gexp b Left) (exp_to_gexp b' Right))) c c' /\
-    holds (interp (gand p (geq (exp_to_gexp b Left) (exp_to_gexp b' Right)))) s0 s0') ==>
-          (terminates_on (reify_computation (while b c)) s0 <==>
-           terminates_on (reify_computation (while b' c')) s0'))
-  = Classical.move_requires (r_while_terminates b b' c c' p s0) s0'
-  in
-  let h (s0 s0':heap) (fuel:nat)
-  :Lemma ((exec_equiv (gand p (gand (exp_to_gexp b Left) (exp_to_gexp b' Right))) (gand p (geq (exp_to_gexp b Left) (exp_to_gexp b' Right))) c c' /\
-    holds (interp (gand p (geq (exp_to_gexp b Left) (exp_to_gexp b' Right)))) s0 s0' /\
-    fst (reify_computation (while b c) fuel s0) == true /\
-    fst (reify_computation (while b' c') fuel s0') == true) ==>
-          (holds (interp (gand p (gnot (gor (exp_to_gexp b Left) (exp_to_gexp b' Right))))) (snd (reify_computation (while b c) fuel s0)) (snd (reify_computation (while b' c') fuel s0'))))
-  = Classical.move_requires (r_while_correct b b' c c' p s0 s0') fuel
-  in
-  Classical.forall_intro_2 g;
-  Classical.forall_intro_3 h
+
+let is_per (p: gexp bool) = Benton2004.is_per (interp p)
 
 (* Aparte: 4.4 How to prove is_per *)
 
-let is_per_geq_exp_to_gexp
+val is_per_geq_exp_to_gexp
   (#t: eqtype)
   (e: exp t)
 : Lemma
   (is_per (geq (exp_to_gexp e Left) (exp_to_gexp e Right)))
-= ()
 
-let is_per_gand_exp_to_gexp
+val is_per_gand_exp_to_gexp
   (b: exp bool)
 : Lemma
   (is_per (gand (exp_to_gexp b Left) (exp_to_gexp b Right)))
-= ()
 
-let is_per_gand
+val is_per_gand
   (e1 e2 : gexp bool)
 : Lemma
   (requires (is_per e1 /\ is_per e2))
   (ensures (is_per (gand e1 e2)))
-= assert (forall s1 s2 .{:pattern (interp (gand e1 e2) s1 s2)} holds (interp (gand e1 e2)) s1 s2 <==> holds (interp e1) s1 s2 /\ holds (interp e2) s1 s2)
 
 (* FIXME: holds but not replayable
 let is_per_gor
@@ -438,29 +424,28 @@ let is_per_gor
 = assert (forall s1 s2 . holds (interp (gor e1 e2)) s1 s2 <==> holds (interp e1) s1 s2 \/ holds (interp e2) s1 s2)
 *)
 
-let r_sym
+val r_sym
   (p p': gexp bool)
   (f f' : computation)
 : Lemma
   (requires (is_per p /\ is_per p'))
   (ensures (exec_equiv p p' f f' <==> exec_equiv p p' f' f))
   [SMTPat (exec_equiv p p' f f'); SMTPat (is_per p); SMTPat (is_per p')]
-= exec_equiv_sym (interp p) (interp p') f f'
+
+let interpolable (p: gexp bool) = Benton2004.interpolable (interp p)
 
 (* Aparte: 4.4 How to prove interpolable *)
 
-let interpolable_geq_exp_to_gexp
+val interpolable_geq_exp_to_gexp
   (#t: eqtype)
   (e: exp t)
 : Lemma
   (interpolable (geq (exp_to_gexp e Left) (exp_to_gexp e Right)))
-= ()
 
-let interpolable_gand_exp_to_gexp
+val interpolable_gand_exp_to_gexp
   (b: exp bool)
 : Lemma
   (interpolable (gand (exp_to_gexp b Left) (exp_to_gexp b Right)))
-= ()
 
 (* FIXME: holds but not replayable
 let interpolable_gand
@@ -478,7 +463,7 @@ let interpolable_gor
 = assert (forall s1 s2 . holds (interp (gor e1 e2)) s1 s2 <==> holds (interp e1) s1 s2 \/ holds (interp e2) s1 s2)
 *)
 
-let r_trans
+val r_trans
   (p p' : gexp bool)
   (c1 c2 c3 : computation)
 : Lemma
@@ -494,20 +479,18 @@ let r_trans
     [SMTPat (exec_equiv p p' c1 c2); SMTPat (exec_equiv p p' c1 c3); SMTPat (is_per p'); SMTPat (interpolable p)];
     [SMTPat (exec_equiv p p' c1 c3); SMTPat (exec_equiv p p' c2 c3); SMTPat (is_per p'); SMTPat (interpolable p)];
   ]]
-= exec_equiv_trans (interp p) (interp p') c1 c2 c3
 
 (* 4.2.1 Basic equations *)
 
-let d_su1
+val d_su1
   (c: computation)
   (phi phi' : gexp bool)
 : Lemma
   (requires (exec_equiv phi phi' c c))
   (ensures (exec_equiv phi phi' (seq skip c) c))
   [SMTPat (exec_equiv phi phi' (seq skip c) c)]
-= Benton2004.d_su1 c (interp phi) (interp phi')
 
-let d_su1'
+val d_su1'
   (c c' c'' : computation)
   (phi phi' phi'' : gexp bool)
 : Lemma
@@ -521,27 +504,24 @@ let d_su1'
     [SMTPat (exec_equiv phi phi'' (seq c c') c''); SMTPat (exec_equiv phi' phi'' c' c'')];
     [SMTPat (exec_equiv phi' phi'' c' c''); SMTPat (exec_equiv phi phi' c skip)];
   ]]
-= Benton2004.d_su1' c c' c'' (interp phi) (interp phi') (interp phi'')
 
-let d_su2
+val d_su2
   (c: computation)
   (phi phi' : gexp bool)
 : Lemma
   (requires (exec_equiv phi phi' c c))
   (ensures (exec_equiv phi phi' (seq c skip) c))
   [SMTPat (exec_equiv phi phi' (seq c skip) c)]
-= Benton2004.d_su2 c (interp phi) (interp phi')
 
-let d_assoc
+val d_assoc
   (c1 c2 c3: computation)
   (phi phi' : gexp bool)
 : Lemma
   (requires (exec_equiv phi phi' (seq (seq c1 c2) c3) (seq (seq c1 c2) c3)))
   (ensures (exec_equiv phi phi' (seq (seq c1 c2) c3) (seq c1 (seq c2 c3))))
   [SMTPat (exec_equiv phi phi' (seq (seq c1 c2) c3) (seq c1 (seq c2 c3)))]
-= Benton2004.d_assoc c1 c2 c3 (interp phi) (interp phi')
 
-let d_cc
+val d_cc
   (b: exp bool)
   (c1 c2 c3: computation)
   (phi phi' phi'' : gexp bool)
@@ -558,31 +538,28 @@ let d_cc
     [SMTPat (exec_equiv phi phi'' (seq (ifthenelse b c1 c2) c3) (ifthenelse b (seq c1 c3) (seq c2 c3))); SMTPat (exec_equiv phi' phi'' c3 c3)];
     [SMTPat (exec_equiv phi phi' (ifthenelse b c1 c2) (ifthenelse b c1 c2)); SMTPat (exec_equiv phi' phi'' c3 c3)];
   ]]
-= Benton2004.d_cc b c1 c2 c3 (interp phi) (interp phi') (interp phi'')
 
-let d_lu1
+val d_lu1
   (b: exp bool)
   (c: computation)
   (phi phi' : gexp bool)
 : Lemma
   (requires (exec_equiv phi phi' (while b c) (while b c)))
   (ensures (exec_equiv phi phi' (while b c) (ifthenelse b (seq c (while b c)) skip)))
-= Benton2004.d_lu1 b c (interp phi) (interp phi')
 
-let d_lu2
+val d_lu2
   (b: exp bool)
   (c: computation)
   (phi phi' : gexp bool)
 : Lemma
   (requires (exec_equiv phi phi' (while b c) (while b c)))
   (ensures (exec_equiv phi phi' (while b c) (while b (seq c (ifthenelse b c skip)))))
-= Benton2004.d_lu2 b c (interp phi) (interp phi')
 
 (* 4.2.2 Optimizing Transformations *)
 
 (* Falsity *)
 
-let r_f
+val r_f
   (c c' : computation)
   (phi: gexp bool)
 : Lemma
@@ -593,11 +570,10 @@ let r_f
       c
       c'
   ))
-= ()
 
 (* Dead assignment *)
 
-let r_dassl
+val r_dassl
   (x: var)
   (e: exp int)
   (phi: gexp bool)
@@ -609,11 +585,10 @@ let r_dassl
       (assign x e)
       skip
   ))
-= ()
 
 (* Common branch *)
 
-let r_cbl
+val r_cbl
   (b: exp bool)
   (c c' d : computation)
   (phi phi' : gexp bool)
@@ -637,19 +612,10 @@ let r_cbl
       (ifthenelse b c c')
       d
   ))
-= (* NOTE: the following let _ are necessary, and must be stated in this form instead of asserts alone, the latter seeming ineffective *)
-  let _ : squash (forall s1 s2 . holds (interp (gand phi (exp_to_gexp b Left))) s1 s2 <==> holds (interp phi) s1 s2 /\ fst (reify_exp b s1) == true) =
-    assert (forall s1 s2 . holds (interp (gand phi (exp_to_gexp b Left))) s1 s2 <==> holds (interp phi) s1 s2 /\ fst (reify_exp b s1) == true)
-  in
-  let _ : squash (forall s1 s2 . holds (interp (gand phi (gnot (exp_to_gexp b Left)))) s1 s2 <==> holds (interp phi) s1 s2 /\ ~ (fst (reify_exp b s1) == true)) =
-    assert (forall s1 s2 . holds (interp (gand phi (gnot (exp_to_gexp b Left)))) s1 s2 <==> holds (interp phi) s1 s2 /\ ~ (fst (reify_exp b s1) == true))
- 
-  in
-  ()
 
 (* Dead while *)
 
-let r_dwhll
+val r_dwhll
   (b: exp bool)
   (c: computation)
   (phi: gexp bool)
@@ -661,4 +627,3 @@ let r_dwhll
       (while b c)
       skip
   ))
-= ()
